---
title: Russell's Paradox, AST and Bears
tags: mathcs, recursion, puremath, logic
---

# Russell's paradox with Sets 

Russell's paradox starts by designing a Set S that contains/specifies all Sets that are not elements of itself. (Note everything in our current model is a set; even the elements of sets are sets)
$$ S = \{ x | x \notin x \} \tag{1}$$
Next we ask can S be an element of S?  
[Assume S is element of itself] 
$$S \in S \tag{2}$$   
[This would imply by definition (1)]
$$S \notin S \tag{3}$$
[By contradiction (2) and (3)]  
$$S \notin S \tag{4}$$

[but by the definition of (1) ]  
$$S \in S \tag{5}$$  
...thus the whole process repeats infinitely  
It is a paradox because there is no end to this proof ( we cannot conclude whether it is true or false )

The resolution is to bound the universe so that S must be within a universe.  

# Russell's paradoxal set S as an AST

![](/images/ycomb/ycombinator.svg)  



# Analogy and Abstracting Russell's paradox with bears
In set theory, the propositional function is elementhood.
Elementhood takes two sets (lets call the universe that contain our sets of interest, $SET$) and return a truth value. Also remember everything is a set.  
We can think of our standard set theory as a pair that contains the universe and it's associated function.
$$(SET,\in)$$

$$ \in :: (SET,SET) \rightarrow bool $$ 



Let's design another theory $$(BEAR, like)$$ with $BEAR$ being defined as the universe of bears.  
$$ like :: (BEAR,BEAR) \rightarrow bool $$

Just like our initial set model, lets pretend everything in our universe is a bear and instead of set containing sets, we have bears liking bears.  

And with theory let's design a paradox using groups of bears and "like".



* Arbitrary bear y that likes bear B iff P(y,likes) is true 
* Arbitrary set x are elements of set S iff P(x,$\in$) is true 
    * where P(x,action) stands for negation of action(x,x) 

Note the similarities between our Set theory and Bear theory.

In other words,  
any bear y must like bear B if and only if bear y does not like itself

# AST with Bears

[Let us define bear B as this AST]  

```plantuml
@startuml
digraph world {
size="3,3";
lbear[label = "lambda-bear"]
bear2[label = "bear"]

lbear -> not 
not -> likes
likes -> bear
likes -> bear2
}
@enduml
```


[bear B likes itself]  
```plantuml
@startuml
digraph world {
size="3,3";
lbear1[label = "lambda-bear"]
lbear2[label = "lambda-bear"]
bear1[label = "bear"]
bear2[label = "bear"]
bear3[label = "bear"]
bear4[label = "bear"]
not1[label = "not"]
not2[label = "not"]
like1[label =  "likes"]
like2[label = "likes"]
like3[label = "likes"]
like1 -> lbear1
like1 -> lbear2
lbear1 -> not1
lbear2 -> not2
not1 -> like2
not2 -> like3
like2 -> bear1
like2 -> bear2
like3 -> bear3
like3 -> bear4
}
@enduml
```


[therefore bear B does not like itself]  
```plantuml
@startuml
digraph world {
size="3,3";
notA[label = "not"]
lbear1[label = "lambda-bear"]
lbear2[label = "lambda-bear"]
bear1[label = "bear"]
bear2[label = "bear"]
bear3[label = "bear"]
bear4[label = "bear"]
not1[label = "not"]
not2[label = "not"]
like1[label =  "likes"]
like2[label = "likes"]
like3[label = "likes"]
notA -> like1
like1 -> lbear1
like1 -> lbear2
lbear1 -> not1
lbear2 -> not2
not1 -> like2
not2 -> like3
like2 -> bear1
like2 -> bear2
like3 -> bear3
like3 -> bear4
}
@enduml
```


[But this means bear B does not not like itself, which is a double negative, meaning bear B likes itself]
```plantuml
@startuml
digraph world {
size="3,3";
notA[label = "not"]
notB[label = "not"]
lbear1[label = "lambda-bear"]
lbear2[label = "lambda-bear"]
bear1[label = "bear"]
bear2[label = "bear"]
bear3[label = "bear"]
bear4[label = "bear"]
not1[label = "not"]
not2[label = "not"]
like1[label =  "likes"]
like2[label = "likes"]
like3[label = "likes"]
notA -> notB
notB -> like1
like1 -> lbear1
like1 -> lbear2
lbear1 -> not1
lbear2 -> not2
not1 -> like2
not2 -> like3
like2 -> bear1
like2 -> bear2
like3 -> bear3
like3 -> bear4
}
@enduml
```


[and so on and so forth...]  
```plantuml
@startuml
digraph world {
size="3,3";
dots[label = "..."]
lbear1[label = "lambda-bear"]
lbear2[label = "lambda-bear"]
bear1[label = "bear"]
bear2[label = "bear"]
bear3[label = "bear"]
bear4[label = "bear"]
not1[label = "not"]
not2[label = "not"]
like1[label =  "likes"]
like2[label = "likes"]
like3[label = "likes"]
dots -> like1
like1 -> lbear1
like1 -> lbear2
lbear1 -> not1
lbear2 -> not2
not1 -> like2
not2 -> like3
like2 -> bear1
like2 -> bear2
like3 -> bear3
like3 -> bear4
}
@enduml
```


## End

Next post will be a short one showcasing the powerful Y-combinator which is closely related to this paradox.  
[Part2 - YCombinator and Recursive  functions](/posts/2018-05-23-YParadox2.html)