---
title: Intro Lean 2
tags: lean, mathcs, puremath ,categorytheory
toc: y
---

# Simp

```hs
@[simp] theorem list.is_prefix_refl (l : list α) : l <+: l :=
⟨[], by simp⟩
```

* The decorator looking like `@[simp]` is actually injecting the theorem into the simp method.
  * This makes simp more powerful
* Lean calls this an ***attribute***

## Simp *

```hs
lemma 
begin
  simp [*]
end
```

* the above simp uses ALL hypothesis in the local context.


# Understanding inductive types

* One can think of terms formed from recursively inductive types as the ROOT of a tree.

```hs
        \     /
        -------- (cons rule)
          \ /
   x::a    y::nlist
    \     /
    -------- (cons rule)
      \ / 
    cons x y :: nlist
```

* Suppose we had an inductive type with no base case
  * it would be non-terminating

```hs
inductive nlist: Type 
 | cons : a -> nlist -> nlist
```

```text
    cons
    / \
   5  cons
      / \
     7  ..inf..
```

**Takeaway: We Must have a NON-RECURSIVE base constructor**  
Heuristic: the recursive type must only appear as the last argument to be considered a non-recursive constructor 

```hs

good1 :: a -> b -> c -> nlist
good2 :: nlist
good3 :: a -> nlist

bad1 :: nlist -> nlist -> a -> nlist
bad2 :: nlist -> nlist
```


# Induction and function definition

```hs
def take {α : Type} : ℕ → list α → list α
| 0       _         := []  --A,B
| (n + 1) []        := []  --C
| (n + 1) (x :: xs) := x :: take n xs --D
```

Below is an inductive proof with leafs labeled as A,B,C,D.

```text
A          B        C           D

ℕ=0,      ℕ=0      ℕ=k-1      ℕ=k-1
list=[]   list=xs   list=[]    list=xs
     \     /            \     / 
      \   /              \   /
   ℕ=0,∀list       ℕ=k-1,∀list     
         \               / 
          \             /
            ∀ℕ ∀list
```

```hs
Proof
  ℕ=n-1
  list=[]
corresponds to 
Code
--            LHS  => RHS + IH             
| (k + 1) []        := []

inductive hypothesis is k,[] which corresponds to ℕ=n-1,list=[]

```

Takeaway:

* The definition of any function is just an inductive proof.